added imperative interface

ParsingNative.cs
@@ -1,7 +1,7 @@
 using System.IO;
 
-namespace @_0_Parsing_Compile {
-  public partial class FileSystem {
+namespace @_0_Internal_Compile {
+  public partial class @FileSystem {
     public static void ReadFile(char[] fname, out char[] result) {
       string sname = new string(fname);
       result = File.ReadAllText(sname).ToCharArray();
