Parsing.dfy
@@ -1,83 +1,184 @@
 module Parsing {
-  datatype Option<A> = Some(some: A) | None
-  datatype Parser<A> = Parser(run: string -> seq<(A, string)>)
+  module Internal {
+    datatype Option<A> = Some(some: A) | None
+    datatype P<A> = P(run: string -> seq<(A, string)>)
 
-  function method SatP(pred: char -> bool): Parser<char>
-  {
-    Parser((s: string) reads pred.reads requires |s| > 0 ==> pred.requires(s[0])
-                       => if |s| == 0 then []
-                          else if pred(s[0]) then [(s[0], s[1..])]
-                          else [])
+    function method SatP(pred: char -> bool): P<char>
+    reads pred.reads;
+    requires forall c:char :: pred.requires(c);
+    ensures forall s:string :: SatP(pred).run.requires(s);
+    {
+      P((s: string) reads pred.reads requires forall c:char :: pred.requires(c)
+                        => if |s| == 0 then []
+                            else if pred(s[0]) then [(s[0], s[1..])]
+                            else [])
+    }
+
+    function method OrP<A>(p1: P<A>, p2: P<A>): P<A>
+    reads p1.run.reads;
+    reads p2.run.reads;
+    requires forall s:string :: p1.run.requires(s);
+    requires forall s:string :: p2.run.requires(s);
+    ensures forall s:string :: OrP(p1, p2).run.requires(s);
+    {
+      P((s: string) reads p1.run.reads reads p2.run.reads
+                    requires p1.run.requires(s) requires p2.run.requires(s)
+                    => p1.run(s) + p2.run(s))
+    }
+
+    function method Map<A,B>(a: seq<A>, f: A -> B): seq<B>
+    reads f.reads;
+    requires forall x: A :: f.requires(x)
+    {
+      if |a| == 0 then []
+                  else [f(a[0])] + Map<A,B>(a[1..], f)
+    }
+
+    function method Flatten<A>(a: seq<seq<A>>): seq<A>
+    {
+      if |a| == 0 then []
+                  else a[0] + Flatten(a[1..])
+    }
+
+    function method ConstP<A>(a: A): P<A>
+    ensures forall s:string :: ConstP(a).run.requires(s) && ConstP(a).run.reads(s) == {};
+    {
+      P((s: string)  => [(a, s)])
+    }
+
+    /* function method ThenP<A,B>(pa: P<A>, pb: A -> P<B>): P<B> */
+    /* reads pa.run.reads; */
+    /* reads pb.reads; */
+    /* requires forall s:string :: pa.run.requires(s); */
+    /* requires forall a:A, s:string :: pb(a).run.requires(s); */
+    /* ensures forall s:string :: ThenP(pa, pb).run.requires(s); */
+    /* { */
+    /*   P((s: string) reads * */
+    /*                 requires pa.run.requires(s) */
+    /*                 requires forall x: A :: pb.requires(x) */
+    /*                 requires forall a: A, s: string :: pb(a).run.requires(s) => */
+    /*   ( */
+    /*     var par: seq<(A, string)> := pa.run(s); */
+    /*     var pcomb: seq<seq<(B, string)>> := Map(par, (a_s: (A, string)) */
+    /*                     reads * */
+    /*                     requires forall x: A :: pb.requires(x) */
+    /*                     requires forall a: A, s: string :: pb(a).run.requires(s) */
+    /*                     => pb(a_s.0).run(a_s.1)); */
+    /*     Flatten(pcomb) */
+    /*   )) */
+    /* } */
+
+    /* function method ZeroOrMoreP<A>(p: P<A>, limit: nat): P<seq<A>> */
+    /* decreases limit */
+    /* { */
+    /*   var nothing: P<seq<A>> := ConstP([]); */
+    /*   if limit == 0 */
+    /*   then nothing */
+    /*   else OrP(nothing, OneOrMoreP<A>(p, limit - 1)) */
+    /* } */
+
+    /* function method OneOrMoreP<A>(p: P<A>, limit: nat): P<seq<A>> */
+    /* decreases limit */
+    /* { */
+    /*   ThenP<A,seq<A>>(p, (a: A) => */
+    /*     if limit == 0 */
+    /*     then ConstP([a]) */
+    /*     else ThenP<seq<A>,seq<A>>(ZeroOrMoreP(p, limit - 1), (aa: seq<A>) => */
+    /*          ConstP([a] + aa))) */
+    /* } */
+
+    class FileSystem {
+      extern static method ReadFile(name:array<char>) returns (contents: array<char>)
+    }
   }
 
-  function method DigitP(): Parser<char>
-  {
-    SatP(c => '0' <= c <= '9')
-  }
+  class Parser<A> {
+    var parser: Internal.P<A>;
 
-  function method LetterP(): Parser<char>
-  {
-    SatP(c => 'A' <= c <= 'Z' || 'a' <= c <= 'z' || c == '_')
-  }
+    constructor (a: A) modifies this
+    requires forall p: Parser<A>, s:string :: p != null ==> p.parser.run.requires(s) && !(this in p.parser.run.reads(s));
+    ensures forall p: Parser<A>, s:string :: p != null ==> p.parser.run.requires(s) && !(this in p.parser.run.reads(s));
+    {
+      parser := Internal.ConstP(a);
+    }
 
-  function method OrP<A>(p1: Parser<A>, p2: Parser<A>): Parser<A>
-  {
-    Parser((s: string) reads p1.run.reads reads p2.run.reads
-                       requires p1.run.requires(s) requires p2.run.requires(s)
-                       => p1.run(s) + p2.run(s))
-  }
+    constructor P(p: Internal.P<A>) modifies this
+    requires forall s:string :: !(this in p.run.reads(s));
+    requires forall s:string :: p.run.requires(s);
+    ensures forall s:string :: parser.run.requires(s);
+    {
+      parser := p;
+    }
 
-  function method Map<A,B>(a: seq<A>, f: A -> B): seq<B>
-  reads f.reads;
-  requires forall x: A :: f.requires(x)
-  {
-    if |a| == 0 then []
-                else [f(a[0])] + Map<A,B>(a[1..], f)
-  }
+    static method Char(c: char) returns (p: Parser<char>)
+    ensures p != null;
+    {
+      return new Parser<char>.P(Internal.SatP(c2 => c == c2));
+    }
 
-  function method Flatten<A>(a: seq<seq<A>>): seq<A>
-  {
-    if |a| == 0 then []
-                else a[0] + Flatten(a[1..])
-  }
+    static method Digit() returns (p: Parser<char>)
+    ensures p != null;
+    ensures forall s:string :: p.parser.run.requires(s);
+    {
+      return new Parser<char>.P(Internal.SatP(c => '0' <= c <= '9'));
+    }
 
-  function method ThenP<A,B>(pa: Parser<A>, pb: A -> Parser<B>): Parser<B>
-  reads *
-  {
-    Parser((s: string) reads *
-                       requires pa.run.requires(s)
-                       requires forall x: A :: pb.requires(x)
-                       requires forall a: A, s: string :: pb(a).run.requires(s) =>
-    (
-      var par: seq<(A, string)> := pa.run(s);
-      var pcomb: seq<seq<(B, string)>> := Map(par, (a_s: (A, string))
-                       reads *
-                       requires forall x: A :: pb.requires(x)
-                       requires forall a: A, s: string :: pb(a).run.requires(s)
-                       => pb(a_s.0).run(a_s.1));
-      Flatten(pcomb)
-    ))
-  }
+    static method Letter() returns (p: Parser<char>)
+    ensures p != null;
+    ensures forall s:string :: p.parser.run.requires(s);
+    {
+      return new Parser<char>.P(Internal.SatP(c => 'A' <= c <= 'Z' || 'a' <= c <= 'z' || c == '_'));
+    }
 
-  class FileSystem {
-    extern static method ReadFile(name:array<char>) returns (contents: array<char>)
-  }
+    /* method Then<B,C>(pb: Parser<B>, f: (A,B) -> C) returns (p: Parser<C>) */
+    /* requires pb != null */
+    /* ensures p != null; */
+    /* { */
+    /*   return new Parser<C>.P(Internal.ThenP(parser, */
+    /*     (a: A) reads pb => Internal.ThenP<B,C>(pb.parser, */
+    /*     (b: B) reads f.reads requires f.requires(a,b) => Internal.ConstP(f(a,b))))); */
+    /* } */
 
-  function method Parse<A>(parser: Parser<A>, str: string): Option<A>
-  reads parser.run.reads;
-  requires forall s : string :: parser.run.requires(s);
-  {
-    var results: seq<(A, string)> := parser.run(str);
-    if |results| == 0 then None else Some(results[0].0)
-  }
+    /* method Or(parser2: Parser<A>) returns (p: Parser<A>) */
+    /* requires parser2 != null */
+    /* ensures p != null; */
+    /* { */
+    /*   return new Parser.P(Internal.OrP(parser, parser2.parser)); */
+    /* } */
 
-  method ParseFile<A>(parser: Parser<A>, filename: string) returns (res: Option<A>)
-  requires forall s : string :: parser.run.requires(s)
-  {
-    var fname: array<char> := new char[|filename|];
-    var contents: array<char> := FileSystem.ReadFile(fname);
-    if contents == null { return None; }
-    var parseResult := Parse(parser, contents[..]);
-    return parseResult;
+    /* method OneOrMore() returns (p: Parser<seq<A>>) */
+    /* ensures p != null; */
+    /* { */
+    /*   return new Parser.P(Internal.ZeroOrMoreP(parser, 1000)); */
+    /* } */
+
+    /* method ZeroOrMore() returns (p: Parser<seq<A>>) */
+    /* ensures p != null; */
+    /* { */
+    /*   return new Parser.P(Internal.OneOrMoreP(parser, 1000)); */
+    /* } */
+
+    function method Parse(str: string): Internal.Option<A>
+    reads this
+    reads parser.run.reads;
+    requires parser.run.requires(str);
+    {
+      var results := parser.run(str);
+      if |results| == 0
+      then Internal.Option.None
+      else Internal.Option.Some(results[0].0)
+    }
+
+    /* method ParseFile(filename: string) returns (res: Internal.Option<A>) */
+    /* requires forall s : string :: parser.run.requires(s) */
+    /* { */
+    /*   var fname: array<char> := new char[|filename|]; */
+    /*   var contents: array<char> := Internal.FileSystem.ReadFile(fname); */
+    /*   if contents == null { return Internal.Option.None; } */
+    /*   assert forall s : string :: parser.run.requires(s); */
+    /*   var parseResult := Parse(contents[..]); */
+    /*   return parseResult; */
+    /* } */
   }
 }
+
