Example.dfy
@@ -4,9 +4,18 @@ module Example {
   import opened Parsing
 
   method Main() {
-    print(Parse(DigitP(), "5")); // Some(5)
-    print(Parse(DigitP(), "X")); // None
-    print(Parse(OrP(DigitP(), LetterP()), "X")); // Some(X)
-    print(Parse(OrP(DigitP(), LetterP()), "+")); // None
+    var digitP := Parser<char>.Digit();
+    var letterP := Parser<char>.Letter();
+    print(digitP.Parse("5")); // Some(5)
+    /* print(digitP.Parse("X")); // None */
+    /* var digitOrLetterP := digitP.Or(letterP); */
+    /* var digitOrLetterSeqP := digitOrLetterP.ZeroOrMore(); */
+
+    /* var idP: Parser<string> := letterP.Then(digitOrLetterSeqP, (c, cs) => [c] + cs); */
+
+    /* print(idP.Parse("x"));   // Some(x) */
+    /* print(idP.Parse("x23")); // Some(X23) */
+    /* print(idP.Parse("A_Z")); // Some(A_Z) */
+    /* print(idP.Parse("12"));  // None */
   }
 }
